<?xml version="1.0"  encoding="UTF-8"?>
<rdf:RDF
    xmlns       ="http://rdf.muninn-project.org/ontologies/cp#"
    xmlns:rdf="http://www.w3.org/1999/02/22-rdf-syntax-ns#"
    xmlns:foaf="http://xmlns.com/foaf/spec/"
    xmlns:dbpedia="http://dbpedia.org/resource/"
    xmlns:skos="http://www.w3.org/2004/02/skos/core#"
    xmlns:time = "http://www.w3.org/2006/time#"
    xmlns:geo="http://www.w3.org/2003/01/geo/wgs84_pos#"
    xmlns:cc = "http://creativecommons.org/ns#"
    xmlns:owl="http://www.w3.org/2002/07/owl#"
    xmlns:olo="http://purl.org/ontology/olo/core#"
    xmlns:vann="http://purl.org/vocab/vann/"
    xmlns:xsd="http://www.w3.org/2001/XMLSchema#"
    xmlns:vs="http://www.w3.org/2003/06/sw-vocab-status/ns#"
    xmlns:swrl="http://www.w3.org/2003/11/swrl#"
    xmlns:dc="http://purl.org/dc/elements/1.1/"
    xmlns:swrlb="http://www.w3.org/2003/11/swrlb#"
    xmlns:rdfs="http://www.w3.org/2000/01/rdf-schema#"
    xml:base="http://rdf.muninn-project.org/ontologies/cp">

  <owl:Ontology rdf:about="">
   <foaf:name>Control Point</foaf:name>
   <dc:title>A simple control point Ontology</dc:title>
   <dc:description>A simple data structure to link up a pixel in an image to a location to warp / reproject a map image.</dc:description>
   <rdfs:label xml:lang="en">Control Point Ontology</rdfs:label>
   <dc:rights rdf:resource="http://creativecommons.org/licenses/by/3.0/"/> 
   <vs:term_status>Testing</vs:term_status>
   <dc:creator rdf:resource="http://rdf.muninn-project.org/ww1/2011/11/11/Person/Warren"/> 
 </owl:Ontology>

 <owl:Class rdf:ID="ControlPoint">
  <foaf:name>ControlPoint</foaf:name>
  <rdfs:label xml:lang="en">ControlPoint</rdfs:label>
  <rdfs:comment xml:lang="en">Relates point in an image to a feature / point in the real world(tm).</rdfs:comment>
 </owl:Class>

<owl:DatatypeProperty rdf:ID="xPixel">
 <foaf:name>X</foaf:name>
 <rdfs:label xml:lang="en">X</rdfs:label>
 <rdfs:comment xml:lang="en">X location of the pixel, index 0, starting from the top left corner of the image.</rdfs:comment>
 <rdfs:domain rdf:resource="ControlPoint"/>
</owl:DatatypeProperty>

<owl:DatatypeProperty rdf:ID="yPixel">
 <foaf:name>Y</foaf:name>
 <rdfs:label xml:lang="en">Y</rdfs:label>
 <rdfs:comment xml:lang="en">Y location of the pixel, index 0, starting from the top left corner of the image.</rdfs:comment>
 <rdfs:domain rdf:resource="ControlPoint"/>
</owl:DatatypeProperty>

<owl:ObjectProperty rdf:ID="feature">
 <foaf:name>Feature</foaf:name>
 <rdfs:label xml:lang="en">Feature</rdfs:label>
 <rdfs:domain rdf:resource="ControlPoint"/>
 <rdfs:comment xml:lang="en">Feature that this control point references. Can be a geometry or a feature with a geometry.</rdfs:comment>  
</owl:ObjectProperty>

<owl:ObjectProperty rdf:ID="image">
 <foaf:name>Image</foaf:name>
 <rdfs:label xml:lang="en">Image</rdfs:label>
 <rdfs:domain rdf:resource="ControlPoint"/>
 <rdfs:comment xml:lang="en">The image that this control point is in.</rdfs:comment>  
</owl:ObjectProperty>

</rdf:RDF>
